theories/stlc/Triangular.v
@@ -1,0 +1,204 @@
+(******************************************************************************)
+(* Copyright (c) 2022 Steven Keuchel                                          *)
+(* All rights reserved.                                                       *)
+(*                                                                            *)
+(* Redistribution and use in source and binary forms, with or without         *)
+(* modification, are permitted provided that the following conditions are     *)
+(* met:                                                                       *)
+(*                                                                            *)
+(* 1. Redistributions of source code must retain the above copyright notice,  *)
+(*    this list of conditions and the following disclaimer.                   *)
+(*                                                                            *)
+(* 2. Redistributions in binary form must reproduce the above copyright       *)
+(*    notice, this list of conditions and the following disclaimer in the     *)
+(*    documentation and/or other materials provided with the distribution.    *)
+(*                                                                            *)
+(* THIS SOFTWARE IS PROVIDED BY THE COPYRIGHT HOLDERS AND CONTRIBUTORS        *)
+(* "AS IS" AND ANY EXPRESS OR IMPLIED WARRANTIES, INCLUDING, BUT NOT LIMITED  *)
+(* TO, THE IMPLIED WARRANTIES OF MERCHANTABILITY AND FITNESS FOR A PARTICULAR *)
+(* PURPOSE ARE DISCLAIMED. IN NO EVENT SHALL THE COPYRIGHT HOLDER OR          *)
+(* CONTRIBUTORS BE LIABLE FOR ANY DIRECT, INDIRECT, INCIDENTAL, SPECIAL,      *)
+(* EXEMPLARY, OR CONSEQUENTIAL DAMAGES (INCLUDING, BUT NOT LIMITED TO,        *)
+(* PROCUREMENT OF SUBSTITUTE GOODS OR SERVICES; LOSS OF USE, DATA, OR         *)
+(* PROFITS; OR BUSINESS INTERRUPTION) HOWEVER CAUSED AND ON ANY THEORY OF     *)
+(* LIABILITY, WHETHER IN CONTRACT, STRICT LIABILITY, OR TORT (INCLUDING       *)
+(* NEGLIGENCE OR OTHERWISE) ARISING IN ANY WAY OUT OF THE USE OF THIS         *)
+(* SOFTWARE, EVEN IF ADVISED OF THE POSSIBILITY OF SUCH DAMAGE.               *)
+(******************************************************************************)
+
+From Em Require Import
+     Definitions Context STLC.
+Import ctx.notations.
+Import SigTNotations.
+
+Set Implicit Arguments.
+
+#[local] Arguments Ty_hole {_ _} _.
+#[local] Arguments Ty_bool {_}.
+#[local] Arguments Ty_func {_}.
+(* #[local] Open Scope indexed_scope. *)
+
+Reserved Notation "w1 ⊒⁻ w2" (at level 80).
+
+Definition Later (A : TYPE) : TYPE :=
+  fun w => forall x (xIn : x ∈ w), A (w - x).
+Definition LaterTm (A : TYPE) : TYPE :=
+  fun w => forall x (xIn : x ∈ w), Ty (w - x) -> A (w - x).
+Notation "▷ A" := (Later A) (at level 9, right associativity).
+Notation "▶ A" := (LaterTm A) (at level 9, right associativity).
+Definition Sooner (A : TYPE) : TYPE :=
+  fun w => sigT (fun x => sigT (fun (xIn : x ∈ w) => A (w - x))).
+Definition SoonerTm (A : TYPE) : TYPE :=
+  fun w => sigT (fun x => sigT (fun (xIn : x ∈ w) => Ty (w - x) * A (w - x)))%type.
+Notation "◁ A" := (Sooner A) (at level 9, right associativity).
+Notation "◀ A" := (SoonerTm A) (at level 9, right associativity).
+
+Section Thick.
+
+  Definition thickIn {w x} (xIn : x ∈ w) (s : Ty (w - x)) :
+    forall y, y ∈ w -> Ty (w - x) :=
+    fun y yIn =>
+      match ctx.occurs_check_view xIn yIn with
+      | ctx.Same _     => s
+      | ctx.Diff _ yIn => Ty_hole yIn
+      end.
+
+  Definition thick : ⊢ Ty -> ▶Ty :=
+    fun w =>
+      fix thick (S : Ty w) (x : nat) (xIn : x ∈ w) (T : Ty (w - x)) {struct S} : Ty (w - x) :=
+      match S with
+      | Ty_hole σIn   => thickIn xIn T σIn
+      | Ty_bool       => Ty_bool
+      | Ty_func S1 S2 => Ty_func (thick S1 x xIn T) (thick S2 x xIn T)
+      end.
+
+End Thick.
+
+Section Thin.
+
+  Fixpoint thin {w x} (xIn : x ∈ w) (T : Ty (w - x)) : Ty w :=
+    match T with
+    | Ty_hole yIn => Ty_hole (ctx.in_thin xIn yIn)
+    | Ty_bool => Ty_bool
+    | Ty_func T1 T2 => Ty_func (thin xIn T1) (thin xIn T2)
+    end.
+
+  Definition fancy_thin : ⊢ ◁Ty -> Ty :=
+    fun w '(x; (xIn; T)) => thin xIn T.
+
+End Thin.
+
+Module Tri.
+
+  Import Coq.Classes.CRelationClasses.
+
+  Inductive Tri (w : World) : World -> Set :=
+  | refl      : w ⊒⁻ w
+  | cons {w' x} (xIn : x ∈ w) (t : Ty (w - x)) (ζ : w - x ⊒⁻ w') : w ⊒⁻ w'
+  where "w1 ⊒⁻ w2" := (Tri w1 w2).
+  Global Arguments refl {_}.
+  Global Arguments cons {_ _} x {_} t ζ.
+
+  Fixpoint trans [w0 w1 w2] (ζ1 : w0 ⊒⁻ w1) {struct ζ1} : w1 ⊒⁻ w2 -> w0 ⊒⁻ w2 :=
+    match ζ1 with
+    | refl        => fun ζ2 => ζ2
+    | cons x t ζ1 => fun ζ2 => cons x t (trans ζ1 ζ2)
+    end.
+  Local Infix "⊙" := trans (at level 60, right associativity).
+  #[export] Instance preorder_tri : PreOrder Tri :=
+    {| PreOrder_Reflexive w := refl;
+       PreOrder_Transitive  := trans
+    |}.
+
+  Definition single {w} x {xIn : x ∈ w} (t : Ty (w - x)) : w ⊒⁻ w - x :=
+    cons x t refl.
+  Global Arguments single {w} x {xIn} t.
+
+  Lemma trans_refl {w1 w2} (ζ : w1 ⊒⁻ w2) : ζ ⊙ refl = ζ.
+  Proof. induction ζ; cbn; congruence. Qed.
+
+  Lemma trans_assoc {w0 w1 w2 w3} (ζ1 : w0 ⊒⁻ w1) (ζ2 : w1 ⊒⁻ w2) (ζ3 : w2 ⊒⁻ w3) :
+    (ζ1 ⊙ ζ2) ⊙ ζ3 = ζ1 ⊙ (ζ2 ⊙ ζ3).
+  Proof. induction ζ1; cbn; congruence. Qed.
+
+  (* Definition geq {w0 w1} (ζ1 : w0 ⊒⁻ w1) [w2] (ζ2 : w0 ⊒⁻ w2) : Prop := *)
+  (*   exists ζ12 : w1 ⊒⁻ w2, ζ2 = ζ1 ⊙ ζ12. *)
+  (* Notation "ζ1 ≽ ζ2" := (geq ζ1 ζ2) (at level 80). *)
+
+  (* Lemma geq_refl {w1 w2} (ζ : w1 ⊒⁻ w2) : ζ ≽ ζ. *)
+  (* Proof. exists refl. symmetry. apply trans_refl. Qed. *)
+
+  (* Lemma geq_trans {w0 w1 w2 w3} (ζ1 : w0 ⊒⁻ w1) (ζ2 : w0 ⊒⁻ w2) (ζ3 : w0 ⊒⁻ w3) : *)
+  (*   ζ1 ≽ ζ2 -> ζ2 ≽ ζ3 -> ζ1 ≽ ζ3. *)
+  (* Proof. *)
+  (*   intros [ζ12 H12] [ζ23 H23]. exists (ζ12 ⊙ ζ23). *)
+  (*   rewrite H23, H12. apply trans_assoc. *)
+  (* Qed. *)
+
+  (* Lemma geq_precom {w0 w1 w2 w3} (ζ1 : w0 ⊒⁻ w1) (ζ2 : w1 ⊒⁻ w2) (ζ3 : w1 ⊒⁻ w3) : *)
+  (*   ζ2 ≽ ζ3 -> ζ1 ⊙ ζ2 ≽ ζ1 ⊙ ζ3. *)
+  (* Proof. intros [ζ23 ->]. exists ζ23. symmetry. apply trans_assoc. Qed. *)
+
+  (* Lemma geq_max {w1 w2} (ζ : w1 ⊒⁻ w2) : refl ≽ ζ. *)
+  (* Proof. exists ζ. reflexivity. Qed. *)
+
+  (* Lemma geq_extend {w0 w1 w2} (ζ1 : w0 ⊒⁻ w1) (ζ2 : w1 ⊒⁻ w2) : ζ1 ≽ ζ1 ⊙ ζ2. *)
+  (* Proof. now exists ζ2. Qed. *)
+
+  (* Definition geqb1 [w0 z] (zIn : z ∈ w0) (tz : Ty (w0 - z)) [w1] (ζ : w0 ⊒⁻ w1) : *)
+  (*   option (w0 - z ⊒⁻ w1). *)
+  (* Proof. *)
+  (*   rename w1 into wend. *)
+  (*   induction ζ. *)
+  (*   + apply None. *)
+  (*   + rename w' into wend. rename t into tx. *)
+  (*     destruct (occurs_check_view xIn zIn). *)
+  (*     * refine (if Ty_eqdec tx tz then Some ζ else None). *)
+  (*     * rename y into z. rename yIn into zIn. *)
+  (*       specialize (IHζ zIn). *)
+  (*       Check (thick (thin _ tz) _ tx). *)
+  (* Admitted. *)
+
+  (* Fixpoint geqb (w0 w1 : World) (ζ1 : w0 ⊒⁻ w1) {w2} (ζ2 : w0 ⊒⁻ w2) {struct ζ1} : *)
+  (*   option (w1 ⊒⁻ w2) := *)
+  (*   match ζ1 with *)
+  (*   | refl => Some ζ2 *)
+  (*   | cons x t__X ζ1' => *)
+  (*       option.bind (geqb1 _ t__X ζ2) (geqb ζ1') *)
+  (*   end. *)
+
+  (* Lemma geqb_spec {w0 w1} (ζ1 : w0 ⊒⁻ w1) : *)
+  (*   forall [w2] (ζ2 : w0 ⊒ˢ w2), *)
+  (*     Bool.reflect (triangular ζ1 ≽ ζ2) (ζ1 ≽? ζ2). *)
+  (* Proof. *)
+  (*   induction ζ1; cbn [geqb triangular]; intros w2 ζ2. *)
+  (*   - constructor. apply geq_max. *)
+  (*   - destruct Ty_eqdec. *)
+  (*     + destruct (IHζ1 _ (thin xIn ⊙ˢ ζ2)); constructor; clear IHζ1. *)
+  (*       * destruct g as [ζ2']. exists ζ2'. *)
+  (*         rewrite comp_assoc. rewrite <- H. clear - e. *)
+  (*         apply env.lookup_extensional. *)
+  (*         intros y yIn. *)
+  (*         rewrite lookup_comp. *)
+  (*         rewrite lookup_thick. unfold thickIn. *)
+  (*         destruct (occurs_check_view xIn yIn). apply e. *)
+  (*         cbn. rewrite lookup_comp. unfold thin. *)
+  (*         now rewrite env.lookup_tabulate. *)
+  (*       * intros [ζ2' ->]. apply n. clear n. exists ζ2'. *)
+  (*         rewrite <- ?comp_assoc. *)
+  (*         rewrite comp_thin_thick. *)
+  (*         rewrite comp_id_left. *)
+  (*         reflexivity. *)
+  (*     + constructor. intros [ζ2' ->]. apply n. clear n. *)
+  (*       rewrite <- ?comp_assoc. *)
+  (*       rewrite comp_thin_thick. *)
+  (*       rewrite comp_id_left. *)
+  (*       cbn. rewrite ?lookup_comp, lookup_thick. *)
+  (*       unfold thickIn. rewrite occurs_check_view_refl. *)
+  (*       now rewrite subst_comp. *)
+  (* Qed. *)
+
+End Tri.
+Export Tri (Tri).
+Notation "w1 ⊒⁻ w2" := (Tri w1 w2) (at level 80).
+Infix "⊙⁻" := Tri.trans (at level 60, right associativity).
